ExistentialRules/ChaseSequence/CoreChase/Homomorphisms.lean
@@ -23,32 +23,32 @@ variable {kb : KnowledgeBase sig}
 namespace CoreChaseBranch
 
 
-  @[grind]
-  theorem exHomFsCore (cb : CoreChaseBranch kb) (n : Nat) (x : CoreChaseNode kb.rules) (x_eq : cb.branch.infinite_list n = some x) :
+  @[grind .]
+  theorem exHomFsCore (cb : CoreChaseBranch kb) (n : Nat) (x : CoreChaseNode kb.rules) (x_eq : x ∈ cb.branch.get? n) :
     ∃ (h : GroundTermMapping sig), h.isHomomorphism x.fs x.core := by
       exact x.core_sse.right
 
-  @[grind]
+  @[grind .]
   theorem exHomPrevCoreToFactSet (cb : CoreChaseBranch kb) (n : Nat) (x y : CoreChaseNode kb.rules)
-    (x_eq : cb.branch.infinite_list n = some x) (y_eq : cb.branch.infinite_list (n + 1) = some y) : ∃ (h : GroundTermMapping sig), h.isHomomorphism x.core y.fs := by
-      have sub : _ := prevCoreSubsetOfFactset cb n x y x_eq y_eq
-      have := GroundTermMapping.exHomSubToSet x.core y.fs sub
+    (x_eq : x ∈ cb.branch.get? n) (y_eq : y ∈ cb.branch.get? (n + 1)) : ∃ (h : GroundTermMapping sig), h.isHomomorphism x.core y.fs := by
+      have sub : x.core ⊆ y.fs := before_core_sub_after_fs cb n x y x_eq y_eq
+      have := x.core.exHomSubToSet y.fs sub
       exact this
 
-  @[grind]
-  theorem exGtmHomSubsetFsCore (cb : CoreChaseBranch kb) (cn : CoreChaseNode kb.rules) (n : Nat) (cn_eq : cb.branch.infinite_list n = some cn) :
+  @[grind .]
+  theorem exGtmHomSubsetFsCore (cb : CoreChaseBranch kb) (cn : CoreChaseNode kb.rules) (n : Nat) (cn_eq : cn ∈ cb.branch.get? n) :
     ∃ (gtm : GroundTermMapping sig), gtm.applyFactSet cn.fs ⊆ cn.core := by
       rcases (exHomFsCore cb n cn cn_eq) with ⟨gtm, gtm_hom⟩
       exists gtm
       intro f f_in
       unfold GroundTermMapping.applyFactSet at f_in
       rcases f_in with ⟨a, ahl, ahr⟩
-      rw [ahr]
+      rw [← ahr]
       apply gtm_hom.right
       apply TermMapping.apply_generalized_atom_mem_apply_generalized_atom_set
       exact ahl
 
-    @[grind]
+  @[grind .]
   theorem exHomCoreSuccCoreIfSuccIsSome (cb : CoreChaseBranch kb) (n : Nat) (x y : CoreChaseNode kb.rules)
     (x_eq : cb.branch.infinite_list n = some x) (y_eq : cb.branch.infinite_list (n + 1) = some y) :
       ∃ (h : GroundTermMapping sig), h.isHomomorphism x.core y.core := by
@@ -59,7 +59,7 @@ namespace CoreChaseBranch
       exists (gtm_yfs_ycore ∘ gtm_xcore_yfs)
       exact GroundTermMapping.isHomomorphism_compose gtm_xcore_yfs gtm_yfs_ycore x.core y.fs y.core gtm_xcore_yfs_hom gtm_yfs_ycore_hom
 
-  @[grind]
+  @[grind .]
   theorem exHomFsSuccFsIfSuccIsSome (cb : CoreChaseBranch kb) (n : Nat) (x y : CoreChaseNode kb.rules)
     (x_eq : cb.branch.infinite_list n = some x) (y_eq : cb.branch.infinite_list (n + 1) = some y) :
       ∃ (h : GroundTermMapping sig), h.isHomomorphism x.fs y.fs := by
@@ -71,25 +71,25 @@ namespace CoreChaseBranch
         exact GroundTermMapping.isHomomorphism_compose gtm_xfs_xcore gtm_xcore_yfs x.fs x.core y.fs gtm_xfs_xcore_hom gtm_xcore_yfs_hom
 
   -- t16 (A_0 → A_1 → A_2 → ...)
-  @[grind]
-  theorem exHomCoreAllFollowingCore (cb : CoreChaseBranch kb) (n : Nat) (x : CoreChaseNode kb.rules) (x_eq : cb.branch.infinite_list n = some x) :
-        ∀ m, (cb.branch.infinite_list (n + m)).is_none_or (fun y => ∃ (h : GroundTermMapping sig), h.isHomomorphism x.core y.core) := by
+  @[grind .]
+  theorem exHomCoreAllFollowingCore (cb : CoreChaseBranch kb) (n : Nat) (x : CoreChaseNode kb.rules) (x_eq : x ∈ cb.branch.get? n) :
+      ∀ m, ∀ y, y ∈ cb.branch.get? (n + m) → ∃ (h : GroundTermMapping sig), h.isHomomorphism x.core y.core := by
       intro m
       induction m with
       | zero =>
-        simp only [Nat.add_zero, Option.is_none_or_iff]
+        simp only [Nat.add_zero, Option.mem_def]
         intro cn cn_eq
         have eq : cn = x := by grind
         exists id
         rw [eq]
-        exact (x.core).id_is_hom
+        exact GroundTermMapping.id_is_hom
       | succ m ih =>
-        rw [Option.is_none_or_iff]
         intro y y_eq
-        simp only [Option.is_none_or_iff] at ih
-        have ex_cm : ∃ (z : CoreChaseNode kb.rules), cb.branch.infinite_list (n + m) = some z := by
-          have := cb.prev_is_some_if_is_some (n+m+1) (Option.NeqNoneIfIsSome (cb.branch.infinite_list (n + m + 1)) y y_eq) (n+m) (Nat.lt_add_one (n + m))
-          exact Option.ne_none_iff_exists'.mp this
+        simp only [Option.mem_def] at ih
+
+        have ex_cm : ∃ (z : CoreChaseNode kb.rules), cb.branch.infinite_list (n + m) = some z :=
+          cb.ex_prev_node_at_each_leq (n + m + 1) (Option.isSome_of_mem y_eq) (n + m) (Nat.le_add_right (n + m) 1)
+
         rcases ex_cm with ⟨z, z_eq⟩
         specialize ih z z_eq
         rcases ih with ⟨gtm_x_z, gtm_x_z_hom⟩
@@ -98,64 +98,47 @@ namespace CoreChaseBranch
         exists (gtm_z_y ∘ gtm_x_z)
         exact GroundTermMapping.isHomomorphism_compose gtm_x_z gtm_z_y x.core z.core y.core gtm_x_z_hom gtm_z_y_hom
 
-  @[grind]
-  theorem exHomFsAllFollowingFs (cb : CoreChaseBranch kb) (n : Nat) (x : CoreChaseNode kb.rules) (x_eq : cb.branch.infinite_list n = some x) :
-        ∀ m, (cb.branch.infinite_list (n + m)).is_none_or (fun y => ∃ (h : GroundTermMapping sig), h.isHomomorphism x.fs y.fs) := by
+  @[grind .]
+  theorem exHomFsAllFollowingFs (cb : CoreChaseBranch kb) (n : Nat) (x : CoreChaseNode kb.rules) (x_eq : x ∈ cb.branch.get? n) :
+        ∀ m, ∀ y, y ∈ cb.branch.get? (n + m) → ∃ (h : GroundTermMapping sig), h.isHomomorphism x.fs y.fs := by
       intro m
       induction m with
       | zero =>
-        simp only [Nat.add_zero, Option.is_none_or]
-        split
-        next => trivial
-        next a b y heq => apply GroundTermMapping.exHomSubToSet x.fs y.fs (by
-          have eq : x = y := by grind
-          rw [eq]
-          apply Set.subset_refl
-          )
+        simp only [Nat.add_zero, Option.mem_def]
+        intro cn cn_eq
+        have eq : cn = x := by grind
+        exists id
+        rw [eq]
+        exact GroundTermMapping.id_is_hom
       | succ m ih =>
-        rw [Option.is_none_or_iff]
         intro y y_eq
-        let prev_node := (cb.prev_node (n + m) (by rw [Nat.add_assoc]; simp [y_eq]))
-        simp only [Option.is_none_or] at ih
-        split at ih
-        next => apply GroundTermMapping.exHomSubToSet x.fs y.fs (by grind)
-        next a b z heq =>
-          have : ∃ (h : GroundTermMapping sig), h.isHomomorphism z.fs y.fs := exHomFsSuccFsIfSuccIsSome cb (n + m) z y heq y_eq
-          rcases ih with ⟨gtm_x_z, gtm_x_z_hom⟩
-          rcases this with ⟨gtm_z_y, gtm_z_y_hom⟩
-          exists (gtm_z_y ∘ gtm_x_z)
-          exact GroundTermMapping.isHomomorphism_compose gtm_x_z gtm_z_y x.fs z.fs y.fs gtm_x_z_hom gtm_z_y_hom
+        let prev_node := cb.prev_node (n + m) (Option.isSome_of_mem y_eq)
+        specialize ih prev_node
+        grind
 
-  @[grind]
+  @[grind .]
   theorem exHomResultIfIsSome (cb : CoreChaseBranch kb) (ter' : cb.terminates') (m : Nat) (cn cn_res : CoreChaseNode kb.rules)
-    (cn_eq : cb.branch.infinite_list m = some cn) (cn_res_eq : cb.branch.infinite_list (cb.last_element_index ter') = some cn_res) :
-    ∃ (h : GroundTermMapping sig), h.isHomomorphism cn.fs cn_res.core := by
+    (cn_eq : cn ∈ cb.branch.get? m) (cn_res_eq : cn_res ∈ cb.branch.get? (cb.last_element_index ter')) :
+      ∃ (h : GroundTermMapping sig), h.isHomomorphism cn.fs cn_res.core := by
+        rcases ter' with ⟨n, term_at_n⟩
+        have ter'_eq : cb.last_element_index (Exists.intro n term_at_n : ∃ n, cb.terminates_at_step n) = n := last_element_index_eq_termintes'_index cb n term_at_n
+        simp only [ter'_eq] at cn_res_eq
+        by_cases case : m < n
+        have := exHomCoreAllFollowingCore cb m cn cn_eq
+        specialize this (n - m)
+        have eq : m + (n - m) = n := by grind
+        grind
+        have case : m = n ∨ m > n:= Nat.eq_or_lt_of_not_lt case
+        cases case with
+          | inl eq =>
+            grind
+          | inr gt =>
+            have contra := CoreChaseBranch.last_element_index_eq_termintes'_index_leq cb n term_at_n m
+            unfold CoreChaseBranch.last_element_index at ter'_eq
+            have := all_succ_of_last_index_none cb n term_at_n m gt
+            grind
 
-      rcases ter' with ⟨n, term_at_n⟩
-      have ter'_eq : cb.last_element_index (Exists.intro n term_at_n : ∃ n, cb.terminates_at_step n) = n := last_element_index_eq_termintes'_index cb n term_at_n
-      simp only [ter'_eq] at cn_res_eq
-      by_cases case : m < n
-      have := exHomCoreAllFollowingCore cb m cn cn_eq
-      specialize this (n - m)
-      have eq : m + (n - m) = n := by grind
-      rw [eq, Option.is_none_or_iff] at this
-      specialize this cn_res cn_res_eq
-      rcases this with ⟨gtm_cn_core_cn_res_core, gtm_cn_core_cn_res_core_hom⟩
-      rcases cn.core_sse.right with ⟨gtm_cn_fs_cn_core, gtm_cn_fs_cn_core_hom⟩
-      exists (gtm_cn_core_cn_res_core ∘ gtm_cn_fs_cn_core)
-      exact GroundTermMapping.isHomomorphism_compose gtm_cn_fs_cn_core gtm_cn_core_cn_res_core cn.fs cn.core cn_res.core gtm_cn_fs_cn_core_hom gtm_cn_core_cn_res_core_hom
-      have case : m = n ∨ m > n:= Nat.eq_or_lt_of_not_lt case
-      cases case with
-        | inl eq =>
-          grind
-        | inr gt =>
-          have contra := CoreChaseBranch.last_element_index_eq_termintes'_index_leq cb n term_at_n m
-          unfold CoreChaseBranch.last_element_index at ter'_eq
-          have := all_succ_of_last_index_none cb n term_at_n m gt
-          rw [cn_eq] at this
-          contradiction
-
-  @[grind]
+  @[grind .]
   theorem homFsToFsAlsoHomCoreToFs (fs : FactSet sig) (cn : CoreChaseNode kb.rules) (h : GroundTermMapping sig) (h_hom : h.isHomomorphism cn.fs fs) : h.isHomomorphism cn.core fs := by
     rcases h_hom with ⟨h_c, h_af⟩
     constructor
@@ -165,10 +148,10 @@ namespace CoreChaseBranch
     apply h_af
     exact GroundTermMapping.memApplyFactSetIfMemApplyFactSetSubSet h cn.core cn.fs f f_in (cn.core_sse.left)
 
-  @[grind]
+  @[grind .]
   theorem gtmFsCoreIsEndo (cb : CoreChaseBranch kb) (cn : CoreChaseNode kb.rules) (n : Nat) (cn_eq : cb.branch.infinite_list n = some cn) (gtm : GroundTermMapping sig) (gtm_hom : gtm.isHomomorphism cn.fs cn.core):
      (gtm.surjective_for_domain_and_image_set cn.core.terms cn.core.terms) := by
-      have sc := FactSet.isStrongCore_of_isWeakCore_of_finite cn.core cn.is_core (all_core_finite cn)
+      have sc := FactSet.isStrongCore_of_isWeakCore_of_finite cn.core cn.is_core (CoreChaseNode.all_core_finite cn)
       specialize sc gtm (homFsToFsAlsoHomCoreToFs cn.core cn gtm gtm_hom)
       rcases sc with ⟨s1, s2, s3⟩
       exact s3
